\documentclass{article}
\usepackage{graphicx}  % for including figures
\usepackage{amsmath,amsthm,amssymb,hyperref,nicematrix, tikz}
\usepackage{arydshln}
\usepackage{mathrsfs}
\usepackage{mathtools}
\usepackage{enumitem}
\usepackage{tikzsymbols}
\usetikzlibrary{tikzmark}
\usepackage{float} % For using H in figure position.
\usepackage{bm}
\usepackage[numbered,framed]{matlab-prettifier}
\usepackage{gensymb}
\usepackage{pgffor}
\usepackage{relsize}
\usepackage{booktabs} % Uses \toprule, midrule, etc. for tables.
\usepackage{caption}
\usepackage{makecell}

\newcommand\independent{\protect\mathpalette{\protect\independenT}{\perp}}

\newcommand{\blue}{\color{blue}}

\NiceMatrixOptions
  {
    custom-line = 
     {
       letter=I, 
       command=hdashedline, 
       tikz=densely dashed,
       width=\pgflinewidth
     },
     cell-space-limits = 1pt
  }

\def\independenT#1#2{\mathrel{\rlap{$#1#2$}\mkern2mu{#1#2}}}
\lstset{style=Matlab-editor}
\newcommand{\R}{\mathbb{R}}
\newcommand{\bigrho}{\raisebox{-.15\baselineskip}{\Large\ensuremath{\rho}}} 

% ------------------------------------------ %
%                   START HERE               %
% ------------------------------------------ %

\begin{document}

Let $\textbf{X}_{1}, \textbf{X}_{2}, \dots, \textbf{X}_{n}$ be a random sample of size $n$ from a $p$-variate normal distribution with mean vector $\bm{\mu}$ and covariance matrix $\bm{\Sigma}$. What's the distribution of (n-1)\textbf{S}?
    \[
        (n-1)\textbf{S}
        =
        \frac{n-1}{n -1}
        \sum_{j=1}^{n}{
            \left(\textbf{X}_{j} - \bar{\textbf{X}}\right)
            {\left(\textbf{X}_{j} - \bar{\textbf{X}}\right)}^{\prime}
        }
        =
    \]
    \[
        =
        \sum_{j=1}^{n}{
            \left(\textbf{X}_{j} + \bm{\mu} - \bm{\mu} - \bar{\textbf{X}}\right)
            {\left(\textbf{X}_{j} + \bm{\mu} - \bm{\mu} - \bar{\textbf{X}}\right)}^{\prime}
        }
        =
    \]
    \[
        =
        \sum_{j=1}^{n}{
            \left((\textbf{X}_{j} - \bm{\mu}) - (\bar{\textbf{X}} - \bm{\mu})\right)
            {\left((\textbf{X}_{j} - \bm{\mu}) - (\bar{\textbf{X}} - \bm{\mu})\right)}^{\prime}
        }
        =
    \]
    \[
        =
        \scriptstyle{
        \sum_{j=1}^{n}{
            (\textbf{X}_{j} - \bm{\mu}){(\textbf{X}_{j} - \bm{\mu})}^{\prime}
            -
            (\bar{\textbf{X}} - \bm{\mu}){(\textbf{X}_{j} - \bm{\mu})}^{\prime}
            -
            (\textbf{X}_{j} - \bm{\mu}){(\bar{\textbf{X}} - \bm{\mu})}^{\prime}
            +
            (\bar{\textbf{X}} - \bm{\mu}){(\bar{\textbf{X}} - \bm{\mu})}^{\prime}
        }
        }
        =
    \]
    \[
        =
        \scriptstyle{
        \sum_{j=1}^{n}{
            (\textbf{X}_{j} - \bm{\mu}){(\textbf{X}_{j} - \bm{\mu})}^{\prime}
        }
        -
        2
        \sum_{j=1}^{n}{
            (\textbf{X}_{j} - \bm{\mu}){(\bar{\textbf{X}} - \bm{\mu})}^{\prime}
        }
        +
        \sum_{j=1}^{n}{
            (\bar{\textbf{X}} - \bm{\mu}){(\bar{\textbf{X}} - \bm{\mu})}^{\prime}
        }
        }
        =
    \]
    \[
        =
        \scriptstyle{
        \sum_{j=1}^{n}{
            (\textbf{X}_{j} - \bm{\mu}){(\textbf{X}_{j} - \bm{\mu})}^{\prime}
        }
        -
        2
        (\bar{\textbf{X}} - \bm{\mu})
        \sum_{j=1}^{n}{
            {(\textbf{X}_{j} - \bm{\mu})}^{\prime}
        }
        +
        n
        (\bar{\textbf{X}} - \bm{\mu}){(\bar{\textbf{X}} - \bm{\mu})}^{\prime}
        }
        =
    \]
    \[
        =
        \scriptstyle{
        \sum_{j=1}^{n}{
            (\textbf{X}_{j} - \bm{\mu}){(\textbf{X}_{j} - \bm{\mu})}^{\prime}
        }
        -
        2
        (\bar{\textbf{X}} - \bm{\mu})
        {((\sum_{j=1}^{n}{\textbf{X}_{j}}) - n\bm{\mu})}^{\prime}
        +
        n
        (\bar{\textbf{X}} - \bm{\mu}){(\bar{\textbf{X}} - \bm{\mu})}^{\prime}
        }
        =
    \]
    \[
        =
        \scriptstyle{
        \sum_{j=1}^{n}{
            (\textbf{X}_{j} - \bm{\mu}){(\textbf{X}_{j} - \bm{\mu})}^{\prime}
        }
        -
        2
        (\bar{\textbf{X}} - \bm{\mu})
        {(n\bar{\textbf{X}} - n\bm{\mu})}^{\prime}
        +
        n
        (\bar{\textbf{X}} - \bm{\mu}){(\bar{\textbf{X}} - \bm{\mu})}^{\prime}
        }
        =
    \]
    \[
        =
        \scriptstyle{
        \sum_{j=1}^{n}{
            (\textbf{X}_{j} - \bm{\mu}){(\textbf{X}_{j} - \bm{\mu})}^{\prime}
        }
        -
        2n
        (\bar{\textbf{X}} - \bm{\mu})
        {(\bar{\textbf{X}} - \bm{\mu})}^{\prime}
        +
        n
        (\bar{\textbf{X}} - \bm{\mu}){(\bar{\textbf{X}} - \bm{\mu})}^{\prime}
        }
        =
    \]
    \[
        =
        \sum_{j=1}^{n}{
            (\textbf{X}_{j} - \bm{\mu}){(\textbf{X}_{j} - \bm{\mu})}^{\prime}
        }
        -
        n
        (\bar{\textbf{X}} - \bm{\mu})
        {(\bar{\textbf{X}} - \bm{\mu})}^{\prime}
        =
    \]
    \[
        =
        \sum_{j=1}^{n}{
            (\textbf{X}_{j} - \bm{\mu}){(\textbf{X}_{j} - \bm{\mu})}^{\prime}
        }
        -
        \left[
            \sqrt{n}
            (\bar{\textbf{X}} - \bm{\mu})
        \right]
        \left[
            \sqrt{n}
            {(\bar{\textbf{X}} - \bm{\mu})}^{\prime}
        \right]
        =
    \]
    so looking at the first and second part of this equation
    \[
        \textbf{X}_{j}
        \sim
        N(\underset{(p \times 1)}{\bm{\mu}}, \underset{(p \times p)}{\bm{\Sigma}})
        \hspace{0.2cm}
        \Rightarrow
        \hspace{0.2cm}
        (\textbf{X}_{j} - \bm{\mu})
        \sim
        N(\textbf{0}, \Sigma)
        \Rightarrow
    \]
    \[
        \Rightarrow
        (\textbf{X}_{j} - \bm{\mu}){(\textbf{X}_{j} - \bm{\mu})}^{\prime}
        \sim
        \chi_{1}^{2}
        \Rightarrow
    \]
    \[
        \Rightarrow
        \sum_{j=1}^{n}{
            (\textbf{X}_{j} - \bm{\mu}){(\textbf{X}_{j} - \bm{\mu})}^{\prime}
        }
        \sim
        W_{p}(n, \Sigma)
    \]
    That is, the first term in the sum is distributed as a Wishart distribution with $n$ degrees of freedom. For the second term,
    \[
        \bar{\textbf{X}}
        \sim
        N(\bm{\mu}, \bm{\Sigma}/n)
        \Rightarrow
        (\bar{\textbf{X}} - \bm{\mu})
        \sim
        N(\textbf{0}, \bm{\Sigma}/n)
        \Rightarrow
    \]
    \[
        \Rightarrow
        \sqrt{n}
        (\bar{\textbf{X}} - \bm{\mu})
        \sim
        N(\textbf{0}, \bm{\Sigma})
        \Rightarrow
    \]
    \[
        \left[
            \sqrt{n}
            (\bar{\textbf{X}} - \bm{\mu})
        \right]
        \left[
            \sqrt{n}
            {(\bar{\textbf{X}} - \bm{\mu})}^{\prime}
        \right]
        \sim
        W_{p}(1, \bm{\Sigma})
    \]

    That is, the second term in the sum is distributed as a Wishart distribution with 1 degree of freedom.

    Combining the two, we now has a Wishart distribution with $n$ degrees of freedom minus another Wishart distribution with 1 degree of freedom to create a Wishart distribution with $n - 1$ distribution, so we finally have
    \[
        (n-1)\textbf{S}
        \sim
        W_{p}\left(n-1, \underset{(p \times p)}{\bm{\Sigma}}\right)
    \]

\end{document}
